Flean/Arith.lean
@@ -1,3 +1,10 @@
 import Flean.Arith.Exceptions
 import Flean.Arith.ULP
 import Flean.Arith.Operations
+import Flean.Arith.Compare
+import Flean.Arith.Sqrt
+import Flean.Arith.FMA
+import Flean.Arith.RoundingHelper
+import Flean.Arith.Conversions
+import Flean.Arith.RoundToIntegral
+import Flean.Arith.Predicates
